\documentclass[fleqn]{article}
\usepackage[utf8]{inputenc}
\usepackage{natbib}
\usepackage{amsmath}
\usepackage{amssymb}
\usepackage{relsize}

\title{\textbf{MATH 307: Individual Homework 20}}
\author{John Mays}
\date{04/21/21, Dr. Guo}

\begin{document}

\maketitle

%\begin{bmatrix}\end{bmatrix}

\section*{Problem 1}
\begin{equation*}
    A = \begin{bmatrix}3&2&1\\6&6&3\\3&0&-1\end{bmatrix}
\end{equation*}
\subsection*{Finding U: }
Row 2: subtract 2 times row 1,\\
Row 3: subtract row 1:
\begin{equation*}
    L_{2}A = \begin{bmatrix}1&0&0\\-2&1&0\\-1&0&1\end{bmatrix}\begin{bmatrix}3&2&1\\6&6&3\\3&0&-1\end{bmatrix} = \begin{bmatrix}3&2&1\\0&2&1\\0&-2&-2\end{bmatrix}
\end{equation*}
Row 3 in new matrix: add row 2
\begin{equation*}
    L_{1}(L_{2}A) =
    \begin{bmatrix}1&0&0\\0&1&0\\0&1&1\end{bmatrix} \begin{bmatrix}3&2&1\\0&2&1\\0&-2&-2\end{bmatrix} = U = \begin{bmatrix}3&2&1\\0&2&1\\0&0&-1\end{bmatrix}
\end{equation*}
\subsection*{Finding L:}
\begin{equation*}
    \begin{split}
    L_{1}L_{2}A &= U = L^{-1}A \implies\\ 
    L^{-1} &= L_{1}L_{2} \implies\\
    L &= (L_{1}L_{2})^{-1} = L_{2}^{-1}L_{1}^{-1} \\
    L &= \begin{bmatrix}1&0&0\\2&1&0\\1&0&1\end{bmatrix}\begin{bmatrix}1&0&0\\0&1&0\\0&-1&1\end{bmatrix} = \begin{bmatrix}1&0&0\\2&1&0\\1&-1&1\end{bmatrix}
    \end{split}
\end{equation*}
\subsection*{Conclusion:}
\begin{equation*}
    A = \begin{bmatrix}3&2&1\\6&6&3\\3&0&-1\end{bmatrix} = LU = \begin{bmatrix}1&0&0\\2&1&0\\1&-1&1\end{bmatrix}\begin{bmatrix}3&2&1\\0&2&1\\0&0&-1\end{bmatrix}
\end{equation*}
\end{document}